src/tls/PNE.fsti
@@ -19,128 +19,140 @@ open Pkg
 
 //let pnlen = 4
 
+type prfid = Flag.prfid
+
+let samplelen = 16
+
+type sample = lbytes samplelen
+
+let safePNE (j:prfid) = Flag.safePNE j
+
+type pne_plainlen = l:nat {l >= 2 /\ l <= 5}
+
+type pne_cipher (l:pne_plainlen) = lbytes l
+
+type pne_cipherpad = lbytes 5
+
+val clip_cipherpad : (cp:pne_cipherpad) -> (l:pne_plainlen) -> pne_cipher l
+// todo write this (slice prefix)
+
+noeq type pne_plain_pkg =
+  | PNEPlainPkg:
+    pne_plain: (j:prfid -> l:pne_plainlen -> (t:Type0{hasEq t})) ->
+    as_bytes: (j:prfid -> l:pne_plainlen -> pne_plain j l -> GTot (lbytes l)) ->
+    repr: (j:prfid{~(safePNE j)} -> l:pne_plainlen -> n:pne_plain j l -> Tot (b:lbytes l{b == as_bytes j l n})) ->
+    pne_plain_pkg
+
+let info = pne_plain_pkg
+
+let pne_plain (u:info) (j:prfid) (l:pne_plainlen) =
+  PNEPlainPkg?.pne_plain u j l
+
+
 val table_region : rgn
 
-let safePNE (i:I.id) = Flag.safePNE i
 
-type cipher = b:bytes{Bytes.length b >= 16}
-
-type ciphersample = lbytes 16
-
-//type pnlen = n:nat{n<=16}
-let pnlen = n:nat{n=1 \/ n=2 \/ n=4}
-
-type epn (l:pnlen) = lbytes l
-
-
-noeq type pn_pkg =
-  | PNPkg:
-    pn: (i:I.id -> l:pnlen -> (t:Type0{hasEq t})) ->
-    as_bytes: (i:I.id -> l:pnlen -> pn i l -> GTot (lbytes l)) ->
-    repr: (i:I.id{~(safePNE i)} -> l:pnlen -> n:pn i l -> Tot (b:lbytes l{b == as_bytes i l n})) ->
-    from_bytes: (i:I.id -> l:pnlen -> b:lbytes l -> GTot (n:pn i l{as_bytes i l n == b})) ->
-    abs: (i:I.id -> l:pnlen -> b:lbytes l -> Tot (n:pn i l{n == from_bytes i l b})) ->
-    pn_pkg
-
-let info = pn_pkg
-
-let pn (i:I.id) (u:info) (l:pnlen) = PNPkg?.pn u i l
-
-let repr (i:I.id{~(safePNE i)}) (u:info) (l:pnlen) (n:pn i u l) = PNPkg?.repr u i l n
-
-let abs (i:I.id{~(safePNE i)}) (u:info) (l:pnlen) (b:lbytes l) = PNPkg?.abs u i l b
-
-type entry (i:I.id) (u:info) =
+type entry (j:prfid) (u:info) =
   | Entry :
-    s:ciphersample ->
-    #l:pnlen -> 
-    ne:epn l ->
-    n:pn i u l ->
-    entry i u
+    s:sample ->
+    #l:pne_plainlen ->
+    n:pne_plain u j l ->
+    c:pne_cipher l ->
+    entry j u
 
-val pne_state : i:I.id -> u:info -> Type0
+val pne_state : (j:prfid) -> (u:info) -> Type0
 
-val table : (#i:I.id) -> (#u:info) -> (st:pne_state i u) -> (h:mem) -> GTot (Seq.seq (entry i u))
+val table : (#j:prfid) -> (#u:info) -> (st:pne_state j u) -> (h:mem) -> GTot (Seq.seq (entry j u))
 
-val footprint : #i:I.id -> #u:info -> st:pne_state i u -> GTot (subrgn table_region)
+val footprint : #j:prfid -> #u:info -> st:pne_state j u -> GTot (subrgn table_region)
 
-val frame_table: #i:I.id -> #u:info -> st:pne_state i u -> l:Seq.seq (entry i u) ->
+val frame_table: #j:prfid -> #u:info -> st:pne_state j u -> l:Seq.seq (entry j u) ->
   h0:mem -> s:Set.set rid -> h1:mem ->
   Lemma
     (requires
-      safePNE i /\
+      safePNE j /\
       table st h0 == l /\
       modifies s h0 h1 /\
       Set.disjoint s (Set.singleton (footprint st)))
     (ensures table st h1 == l)
 
-let sample_filter (i:I.id) (u:info) (s:ciphersample) (e:entry i u) : bool =
+let sample_filter (j:prfid) (u:info) (s:sample) (e:entry j u) : bool =
   Entry?.s e = s
 
-let entry_for_sample (#i:I.id) (#u:info) (s:ciphersample) (st:pne_state i u) (h:mem) :
-  GTot (option (entry i u)) =
-  Seq.find_l (sample_filter i u s) (table st h)
+let entry_for_sample (#j:prfid) (#u:info) (s:sample) (st:pne_state j u) (h:mem) :
+  GTot (option (entry j u)) =
+  Seq.find_l (sample_filter j u s) (table st h)
   
-let fresh_sample (#i:I.id) (#u:info) (s:ciphersample) (st:pne_state i u) (h:mem) :
+let fresh_sample (#j:prfid) (#u:info) (s:sample) (st:pne_state j u) (h:mem) :
   GTot bool =
   None? (entry_for_sample s st h)
 
-let find_sample (#i:I.id) (#u:info) (s:ciphersample) (st:pne_state i u) (h:mem) :
+let find_sample (#j:prfid) (#u:info) (s:sample) (st:pne_state j u) (h:mem) :
   GTot bool =
   Some? (entry_for_sample s st h)
 
 
-let sample_epn_filter (i:I.id) (u:info) (s:ciphersample) (#l:pnlen) (ne:epn l) (e:entry i u) : bool =
-  Entry?.s e = s && Entry?.l e = l && Entry?.ne e = ne
+let sample_cipher_filter (j:prfid) (u:info) (s:sample) (#l:pne_plainlen) (c:pne_cipher l) (e:entry j u) : bool =
+  Entry?.s e = s && Entry?.l e = l && Entry?.c e = c
 
-let entry_for_sample_epn (#i:I.id) (#u:info) (s:ciphersample) (#l:pnlen) (ne:epn l) (st:pne_state i u) (h:mem) :
-  GTot (option (entry i u)) =
-  Seq.find_l (sample_epn_filter i u s #l ne) (table st h)
+let entry_for_sample_cipher (#j:prfid) (#u:info) (s:sample) (#l:pne_plainlen) (c:pne_cipher l) (st:pne_state j u) (h:mem) :
+  GTot (option (entry j u)) =
+  Seq.find_l (sample_cipher_filter j u s #l c) (table st h)
   
-let find_sample_epn (#i:I.id) (#u:info) (s:ciphersample) (#l:pnlen) (ne:epn l) (st:pne_state i u) (h:mem) :
+let find_sample_cipher (#j:prfid) (#u:info) (s:sample) (#l:pne_plainlen) (c:pne_cipher l) (st:pne_state j u) (h:mem) :
   GTot bool =
-  Some? (entry_for_sample_epn s ne st h)
+  Some? (entry_for_sample_cipher s #l c st h)
+
+let sample_cipherpad_filter (j:prfid) (u:info) (s:sample) (cp:pne_cipherpad) (e:entry j u) : bool =
+  Entry?.s e = s && clip_cipherpad cp (Entry?.l e) = Entry?.c e
+
+let entry_for_sample_cipherpad (#j:prfid) (#u:info) (s:sample) (cp:pne_cipherpad) (st:pne_state j u) (h:mem) :
+  GTot (option (entry j u)) =
+  Seq.find_l (sample_cipherpad_filter j u s cp) (table st h)
+  
+let find_sample_cipherpad (#j:prfid) (#u:info) (s:sample) (cp:pne_cipherpad) (st:pne_state j u) (h:mem) :
+  GTot bool =
+  Some? (entry_for_sample_cipher s cp st h)
 
 
-let sample_cipher (c:cipher) : s:ciphersample =
-  Bytes.slice c 0ul 16ul
-
-val create (i:I.id) (u:info) : ST (pne_state i u)
+val create (j:prfid) (u:info) : ST (pne_state j u)
   (requires fun _ -> True)
   (ensures fun h0 st h1 ->
     modifies_none h0 h1 /\
     table st h1 == Seq.empty)
 
+
 val encrypt :
-  (#i:I.id) ->
+  (#j:prfid) ->
   (#u:info) ->
-  (st:pne_state i u) ->
-  (#l:pnlen) ->
-  (n:pn i u l) ->
-  (s:ciphersample) ->
-  ST (epn l)
+  (st:pne_state j u) ->
+  (#l:pne_plainlen) ->
+  (n:pne_plain u j l) ->
+  (s:sample) ->
+  ST (pne_cipher l)
   (requires fun h0 ->
     fresh_sample s st h0)
-  (ensures fun h0 ne h1 ->
+  (ensures fun h0 c h1 ->
     modifies_one (footprint st) h0 h1 /\
-    (safePNE i ==> table st h1 == Seq.snoc (table st h0) (Entry s ne n)))
+    (safePNE j ==>
+      table st h1 == Seq.snoc (table st h0) (Entry s #l n c)))
 
 #reset-options "--z3rlimit 50"
+
 val decrypt :
-  (#i:I.id) ->
-  (#u: info) ->
-  (st:pne_state i u) ->
-  (#l:pnlen) ->
-  (ne:epn l) ->
-  (s:ciphersample) ->
-  ST (pn i u l)
+  (#j:prfid) ->
+  (#u:info) ->
+  (st:pne_state j u) ->
+  (cp:pne_cipherpad) ->
+  (s:sample) ->
+  ST (l:pne_plainlen & pne_plain u j l)
   (requires fun h0 -> True)
-  (ensures fun h0 n h1 ->
+  (ensures fun h0 (|l, n|) h1 ->
     modifies_none h0 h1 /\
-    ((safePNE i /\ find_sample s st h0) ==>
+    ((safePNE j /\ find_sample s st h0) ==>
      (match entry_for_sample s st h0 with
-        | Some (Entry _ #l' ne' n') -> (l = l' /\ n = n') <==> (l = l' /\ ne = ne'))
+        | Some (Entry _ #l' n' c') ->
+        (l = l' /\ n = n') <==>
+        (l = l' /\ c' = clip_cipherpad cp l))
     )
-  )
-
-
+  ) 
