src/tls/QUICStream.fsti
@@ -14,113 +14,153 @@ open Mem
 open Pkg
 
 
-let safeId (i:I.id) = AEAD.safeId i
-let safePNE (j:I.id) = PNE.safePNE j
+type prfid = Flag.prfid
+type quicid = Flag.quicid
 
-type plainLen = l:nat{l + v AEAD.taglen <= pow2 32 - 1 /\ l + v AEAD.taglen >= 16}
+let safeId (i:I.id) = Flag.safeId i
+let safePNE (j:prfid) = Flag.safePNE j
+let safeQUIC (k:quicid) = Flag.safeQUIC k
 
-type cipher (i:I.id) (l:plainLen) = lbytes (l + v AEAD.taglen)
+type pnlen = nl:nat{nl >= 1 /\ nl <= 4}
+
+type headerlen = hl:nat{hl >= 1 /\ hl <= pow2 32 - 1}
+
+type quic_header (k:quicid) (hl:headerlen) =
+  | Short_header: (b:lbytes hl) -> quic_header k hl
+  | Long_header: (b:lbytes hl) -> quic_header k hl
+
+let bytes_of_quic_header (#k:quicid) (#hl:headerlen) (hd:quic_header k hl) : lbytes hl =
+  match hd with
+    | Short_header b -> b
+    | Long_header b -> b
+
+let pne_plain (j:prfid) (l:PNE.pne_plainlen) : (t:Type0{hasEq t}) = lbytes l
+
+let pne_as_bytes (j:prfid) (l:PNE.pne_plainlen) (n:pne_plain j l) : GTot (lbytes l) = n
+
+let pne_repr (j:prfid {~ (safePNE j)}) (l:PNE.pne_plainlen) (n:pne_plain j l) :
+  Tot (b:lbytes l{b == pne_as_bytes j l n}) = n
+
+#reset-options "--z3rlimit 50"
+
+let pne_plain_pkg = PNE.PNEPlainPkg pne_plain pne_as_bytes pne_repr
+
+let samplelen = 16
+
+type plainlen = l:nat{l + v AEAD.taglen <= pow2 32 - 1}
+
+type pnplainlen = l:nat{l + v AEAD.taglen <= pow2 32 - 1 /\ l + v AEAD.taglen >= samplelen + 4}
+
+type quic_protect (k:quicid) (l:pnplainlen) =
+  lbytes (l + v AEAD.taglen) 
+
+type quic_packet (k:quicid) (hl:headerlen) (l:pnplainlen{hl + l + v AEAD.taglen <= pow2 32 - 1}) =
+  quic_header k hl * quic_protect k l
+
+type cipher (i:I.id) (l:plainlen) = lbytes (l + v AEAD.taglen)
 
 let max_ctr = pow2 62 - 1
 
 
 (* plain pkg *)
-val plain: i:I.id -> l:plainLen -> t:Type0{hasEq t}
+val plain: i:I.id -> l:plainlen -> t:Type0{hasEq t}
 
-val plain_as_bytes : i:I.id -> l:plainLen -> p:plain i l -> GTot (lbytes l)
+val plain_as_bytes : i:I.id -> l:plainlen -> p:plain i l -> GTot (lbytes l)
 
-val mk_plain: i:I.id -> l:plainLen -> b:lbytes l -> p:plain i l{~(AEAD.safeId i) ==> plain_as_bytes i l p == b}
+val mk_plain: i:I.id -> l:plainlen -> b:lbytes l -> p:plain i l{~(AEAD.safeId i) ==> plain_as_bytes i l p == b}
 
-val plain_repr : i:I.id{~(AEAD.safeId i)} -> l:plainLen -> p:plain i l -> b:lbytes l{b == plain_as_bytes i l p}
+val plain_repr : i:I.id{~(AEAD.safeId i)} -> l:plainlen -> p:plain i l -> b:lbytes l{b == plain_as_bytes i l p}
 
 let aead_plain_pkg = AEAD.PlainPkg 0 plain plain_as_bytes plain_repr
 
+type qiv (k:quicid) = AEAD.iv (I.cipherAlg_of_id (fst k))
 
 (* nonce pkg *)
-let pnlen = n:nat{n=1 \/ n=2 \/ n=4}
 
-val nonce (i:I.id) (nl:pnlen) : (t:Type0{hasEq t})
+val nonce (i:I.id) : (t:Type0{hasEq t})
 
-val nonce_as_bytes (i:I.id) (nl:pnlen) (n:nonce i nl) : GTot (AEAD.iv (I.cipherAlg_of_id i))
+val nonce_as_bytes (i:I.id) (n:nonce i) : GTot (AEAD.iv (I.cipherAlg_of_id i))
 
-val nonce_repr (i:I.id{~(safeId i)}) (nl:pnlen) (n:nonce i nl) :
-  Tot (b:AEAD.iv (I.cipherAlg_of_id i){b == nonce_as_bytes i nl n})
+val nonce_repr (i:I.id{~(safeId i)}) (n:nonce i) :
+  Tot (b:AEAD.iv (I.cipherAlg_of_id i){b == nonce_as_bytes i n})
 
 let aead_nonce_pkg =
-  AEAD.NoncePkg pnlen nonce nonce_as_bytes nonce_repr
+  AEAD.NoncePkg nonce nonce_as_bytes nonce_repr
 
 
-(* pn pkg *)
-val npn: j:I.id -> l:pnlen -> t:Type0{hasEq t}
+type sample = PNE.sample
 
-val npn_as_bytes : j:I.id -> l:pnlen -> n:npn j l -> GTot (lbytes l)
-
-val mk_npn: j:I.id -> l:pnlen -> b:lbytes l -> n:npn j l{~(PNE.safePNE j) ==> npn_as_bytes j l n == b}
-
-val npn_repr : j:I.id{~(PNE.safePNE j)} -> l:pnlen -> n:npn j l -> b:lbytes l{b == npn_as_bytes j l n}
-
-val npn_from_bytes : j:I.id -> l:pnlen -> b:lbytes l -> GTot (n:npn j l{npn_as_bytes j l n == b}) 
-
-val npn_abs : j:I.id{~(PNE.safePNE j)} -> l:pnlen -> b:lbytes l -> Tot (n:npn j l{n == npn_from_bytes j l b})
-  
-let npn_pkg = PNE.PNPkg npn npn_as_bytes npn_repr npn_from_bytes npn_abs
-
-
-
-let epn = PNE.epn
+type epn (nl:pnlen) = lbytes nl
 
 type rpn = n:U64.t{U64.v n <= max_ctr}
 
 let rpn_of_nat (j:nat{j<= max_ctr}) : rpn =
   U64.uint_to_t j
 
+type npn (j:prfid) (nl:pnlen) = lbytes nl
 
-val npn_encode : (j:I.id) -> (r:rpn) -> (l:pnlen) -> (n:npn j l)
+//get the first byte of the (unprotected) header + the pn = what needs to be protected by pne
+val pne_plain_of_header_pn (#k:quicid) (#hl:headerlen) (hd:quic_header k hl) (#nl:pnlen) (n:npn (snd k) nl) :  pne_plain (snd k) (nl+1)
 
-val npn_decode : (#j:I.id) -> (#nl:pnlen) -> (n:npn j nl) -> (expected_pn:rpn) -> rpn
+//reconstruct the unprotected header (using the protected header), and the pn, from the protected header and pn
+val header_pn_of_pne_plain (#k:quicid) (#hl:headerlen) (ph:quic_header k hl) (#ll:PNE.pne_plainlen) (pp:pne_plain (snd k) ll) : quic_header k hl * npn (snd k) (ll-1)
+
+//val pheader_epn_of_pne_cipher (#k:quicid) (#hl:headerlen) (hd:quic_header k hl) (l:PNE.pne_plainlen) (c:PNE.pne_cipher l) : quic_header k hl * (nl:pnlen & epn nl)
+
+//get the protected first byte from the (protected) header + the epn = a cipher for pne
+val pne_cipher_of_pheader_epn (#k:quicid) (#hl:headerlen) (ph:quic_header k hl) (#nl:pnlen) (ne:epn nl) :
+  c:PNE.pne_cipher (nl + 1)
+
+//get the pne ciphertext assuming the largest possible pn length (ie 4)
+val pne_cipherpad_of_pheader_quicprotect (#k:quicid) (#hl:headerlen) (ph:quic_header k hl) (#nll:pnplainlen) (qp:quic_protect k nll) :
+  c:PNE.pne_cipherpad
+
+val npn_encode : (j:prfid) -> (r:rpn) -> (nl:pnlen) -> (n:npn j nl)
+
+val npn_decode : (#j:prfid) -> (#nl:pnlen) -> (n:npn j nl) -> (expected_pn:rpn) -> rpn
 
 val create_nonce : #i:I.id -> #alg:I.cipherAlg{alg == I.cipherAlg_of_id i} ->
-  iv: AEAD.iv alg -> nl:pnlen -> r:rpn -> Tot (nonce i nl)
+  iv: AEAD.iv alg -> r:rpn -> Tot (nonce i)
 
 
-val stream_writer: (i:I.id) -> (j:I.id) -> Type0
-val stream_reader: #i:I.id -> #j:I.id -> w:stream_writer i j -> Type0
+val stream_writer: (k:quicid) -> Type0
+val stream_reader: #k:quicid -> w:stream_writer k -> Type0
 
-val writer_aead_state : #i:I.id -> #j:I.id -> w:stream_writer i j ->
-  aw:AEAD.aead_writer i
+val writer_aead_state : (#k:quicid) -> (w:stream_writer k) ->
+  aw:AEAD.aead_writer (fst k)
   {(AEAD.wgetinfo aw).AEAD.plain == aead_plain_pkg /\
   (AEAD.wgetinfo aw).AEAD.nonce == aead_nonce_pkg} 
-val reader_aead_state : #i:I.id -> #j:I.id -> #w:stream_writer i j -> r:stream_reader w ->
+val reader_aead_state : #k:quicid -> #w:stream_writer k -> r:stream_reader w ->
   ar:AEAD.aead_reader (writer_aead_state w)
   {(AEAD.rgetinfo ar).AEAD.plain == aead_plain_pkg /\
   (AEAD.rgetinfo ar).AEAD.nonce == aead_nonce_pkg} 
 
-val writer_pne_state : #i:I.id -> #j:I.id -> w:stream_writer i j -> PNE.pne_state j npn_pkg
-val reader_pne_state : #i:I.id -> #j:I.id -> #w:stream_writer i j -> r:stream_reader w -> PNE.pne_state j npn_pkg
+val writer_pne_state : #k:quicid -> w:stream_writer k -> PNE.pne_state (snd k) pne_plain_pkg
+val reader_pne_state : #k:quicid -> #w:stream_writer k -> r:stream_reader w -> PNE.pne_state (snd k) pne_plain_pkg
 
-val invariant: #i:I.id -> #j:I.id -> w:stream_writer i j -> h:mem ->
+val invariant: #k:quicid -> w:stream_writer k -> h:mem ->
   t:Type0{t ==> AEAD.winvariant (writer_aead_state w) h} 
-val rinvariant: #i:I.id -> #j:I.id -> #w:stream_writer i j -> r:stream_reader w -> h:mem ->
+val rinvariant: #k:quicid -> #w:stream_writer k -> r:stream_reader w -> h:mem ->
   t:Type0{t ==> AEAD.winvariant (writer_aead_state w) h} 
 
-val wctrT: #i:I.id -> #j:I.id -> w:stream_writer i j -> mem -> GTot (n:nat{n<=max_ctr})
-val wctr: #i:I.id -> #j:I.id -> w:stream_writer i j -> ST rpn
+val wctrT: #k:quicid -> w:stream_writer k -> mem -> GTot (n:nat{n<=max_ctr})
+val wctr: #k:quicid -> w:stream_writer k -> ST rpn
   (requires fun h0 -> True)
   (ensures fun h0 c h1 -> h0 == h1 /\ UInt64.v c = wctrT w h1)
 
-val writer_iv: #i:I.id -> #j:I.id -> w:stream_writer i j -> AEAD.iv (I.cipherAlg_of_id i)
-val reader_iv: #i:I.id -> #j:I.id -> #w:stream_writer i j -> r:stream_reader w ->
-  iv:AEAD.iv (I.cipherAlg_of_id i){iv = writer_iv w}
+val writer_iv: #k:quicid -> w:stream_writer k -> qiv k
+val reader_iv: #k:quicid -> #w:stream_writer k -> r:stream_reader w ->
+  iv:qiv k{iv = writer_iv w}
 
-val expected_pnT: #i:I.id -> #j:I.id -> #w:stream_writer i j -> r:stream_reader w -> h:mem ->
+val expected_pnT: #k:quicid -> #w:stream_writer k -> r:stream_reader w -> h:mem ->
   GTot rpn
-val expected_pn: #i:I.id -> #j:I.id -> #w:stream_writer i j -> r:stream_reader w -> ST rpn
+val expected_pn: #k:quicid -> #w:stream_writer k -> r:stream_reader w -> ST rpn
   (requires fun h0 -> True)
   (ensures fun h0 c h1 -> h0 == h1 /\
-    (c == expected_pnT #i #j #w r h0))
+    (c == expected_pnT #k #w r h0))
 
 
-let wincrementable (#i:I.id) (#j:I.id) (w:stream_writer i j) (h:mem) =
+let wincrementable (#k:quicid) (w:stream_writer k) (h:mem) =
   wctrT w h < max_ctr
 
 
@@ -132,20 +172,20 @@ type info' = {
   parent: subrgn tls_tables_region;
 }
 
-type info (i:I.id) (j:I.id) =
-  info:info'{I.aeadAlg_of_id i == info.alg}
+type info (k:quicid) =
+  info:info'{I.aeadAlg_of_id (fst k) == info.alg}
 
-val shared_footprint: #i:I.id -> #j:I.id -> w:stream_writer i j -> GTot rset
+val shared_footprint: #k:quicid -> w:stream_writer k -> GTot rset
 
-val footprint: #i:I.id -> #j:I.id -> w:stream_writer i j -> GTot (s:rset{Set.disjoint s (shared_footprint w)})
+val footprint: #k:quicid -> w:stream_writer k -> GTot (s:rset{Set.disjoint s (shared_footprint w)})
 
-let rshared_footprint (#i:I.id) (#j:I.id) (#w:stream_writer i j) (r:stream_reader w): GTot rset =
+let rshared_footprint (#k:quicid) (#w:stream_writer k) (r:stream_reader w): GTot rset =
   shared_footprint w
 
-val rfootprint: #i:I.id -> #j:I.id -> #w:stream_writer i j -> r:stream_reader w -> GTot (s:rset{Set.disjoint s (rshared_footprint r)})
+val rfootprint: #k:quicid -> #w:stream_writer k -> r:stream_reader w -> GTot (s:rset{Set.disjoint s (rshared_footprint r)})
  
 
-val frame_invariant: #i:I.id -> #j:I.id -> w:stream_writer i j -> h0:mem -> ri:rid -> h1:mem ->
+val frame_invariant: #k:quicid -> w:stream_writer k -> h0:mem -> ri:rid -> h1:mem ->
   Lemma
   (requires
     (invariant w h0 /\
@@ -154,7 +194,7 @@ val frame_invariant: #i:I.id -> #j:I.id -> w:stream_writer i j -> h0:mem -> ri:r
     ~(Set.mem ri (shared_footprint w))))
   (ensures invariant w h1)
 
-val rframe_invariant: #i:I.id -> #j:I.id -> #w:stream_writer i j -> r:stream_reader w -> h0:mem -> ri:rid -> h1:mem ->
+val rframe_invariant: #k:quicid -> #w:stream_writer k -> r:stream_reader w -> h0:mem -> ri:rid -> h1:mem ->
   Lemma
   (requires
     (rinvariant r h0 /\
@@ -164,11 +204,10 @@ val rframe_invariant: #i:I.id -> #j:I.id -> #w:stream_writer i j -> r:stream_rea
   (ensures rinvariant r h1)
 
 
-val wframe_log: #i:I.id{safeId i} -> #j:I.id -> w:stream_writer i j -> l:Seq.seq (AEAD.entry i (AEAD.wgetinfo (writer_aead_state w))) ->
+val wframe_log: #k:quicid{safeId (fst k)} -> w:stream_writer k -> l:Seq.seq (AEAD.entry (fst k) (AEAD.wgetinfo (writer_aead_state w))) ->
   h0:mem -> ri:rid -> h1:mem ->
   Lemma
   (requires
-    Flag.safeId i /\
     invariant w h0 /\
     AEAD.wlog (writer_aead_state w) h0 == l /\
     modifies_one ri h0 h1 /\
@@ -176,11 +215,10 @@ val wframe_log: #i:I.id{safeId i} -> #j:I.id -> w:stream_writer i j -> l:Seq.seq
     ~(Set.mem ri (shared_footprint w)))
   (ensures invariant w h1 ==> AEAD.wlog (writer_aead_state w) h1 == l)
 
-val rframe_log: #i:I.id{safeId i} -> #j:I.id -> #w:stream_writer i j -> r:stream_reader w -> l:Seq.seq (AEAD.entry i (AEAD.rgetinfo (reader_aead_state r))) ->
+val rframe_log: #k:quicid{safeId (fst k)} -> #w:stream_writer k -> r:stream_reader w -> l:Seq.seq (AEAD.entry (fst k) (AEAD.rgetinfo (reader_aead_state r))) ->
   h0:mem -> ri:rid -> h1:mem ->
   Lemma
   (requires
-    Flag.safeId i /\
     invariant w h0 /\
     AEAD.rlog (reader_aead_state r) h0 == l /\
     modifies_one ri h0 h1 /\
@@ -189,22 +227,22 @@ val rframe_log: #i:I.id{safeId i} -> #j:I.id -> #w:stream_writer i j -> r:stream
   (ensures invariant w h1 ==> AEAD.rlog (reader_aead_state r) h1 == l)
 
 
-val wframe_pnlog: #i:I.id -> #j:I.id -> w:stream_writer i j -> l:Seq.seq (PNE.entry j npn_pkg) ->
+val wframe_pnlog: #k:quicid -> w:stream_writer k -> l:Seq.seq (PNE.entry (snd k) pne_plain_pkg) ->
   h0:mem -> ri:rid -> h1:mem ->
   Lemma
   (requires
-    Flag.safePNE j /\
+    safePNE (snd k) /\
     PNE.table (writer_pne_state w) h0 == l /\
     modifies_one ri h0 h1 /\
     ~(Set.mem ri (footprint w)) /\
     ~(Set.mem ri (shared_footprint w)))
   (ensures PNE.table (writer_pne_state w) h1 == l)
 
-val rframe_pnlog: #i:I.id -> #j:I.id -> #w:stream_writer i j -> r:stream_reader w -> l:Seq.seq (PNE.entry j npn_pkg) ->
+val rframe_pnlog: #k:quicid ->  #w:stream_writer k -> r:stream_reader w -> l:Seq.seq (PNE.entry (snd k) pne_plain_pkg) ->
   h0:mem -> ri:rid -> h1:mem ->
   Lemma
   (requires
-    Flag.safePNE j /\
+    safePNE (snd k) /\
     PNE.table (reader_pne_state r) h0 == l /\
     modifies_one ri h0 h1 /\
     ~(Set.mem ri (rfootprint r)) /\
@@ -212,15 +250,15 @@ val rframe_pnlog: #i:I.id -> #j:I.id -> #w:stream_writer i j -> r:stream_reader 
   (ensures PNE.table (reader_pne_state r) h1 == l)
 
 
-val create: i:I.id -> j:I.id -> u:info i j ->
-  ST (stream_writer i j)
+val create: k:quicid -> u:info k ->
+  ST (stream_writer k)
   (requires fun h0 -> 
     disjoint u.shared u.local)
   (ensures fun h0 w h1 ->
     invariant w h1 /\
     shared_footprint w == Set.singleton u.shared /\
     modifies_none h0 h1 /\
-    (Flag.safeId i /\ Flag.safePNE j) ==>
+    (safeId (fst k) /\ safePNE (snd k)) ==>
     (AEAD.wlog (writer_aead_state w) h1 == Seq.empty /\
     PNE.table (writer_pne_state w) h1 == Seq.empty /\
     wctrT w h1 == 0)
@@ -237,77 +275,101 @@ val create: i:I.id -> j:I.id -> u:info i j ->
     modifies_none h0 h1)
 *)
 
-val createReader: parent:rgn -> #i:I.id -> #j:I.id -> w:stream_writer i j ->
+val createReader: parent:rgn -> #k:quicid -> w:stream_writer k ->
   ST (stream_reader w)
   (requires fun h0 -> invariant w h0)
   (ensures fun h0 r h1 ->
     invariant w h1 /\
     rinvariant r h1 /\
     modifies_none h0 h1 /\
-    (Flag.safeId i /\ Flag.safePNE j) ==>
+    (safeId (fst k) /\ safePNE (snd k)) ==>
       expected_pnT r h1 == U64.uint_to_t 0)
+
+//split the epn+cipher, given the length of the epn
+val split (#k:quicid) (#l:pnplainlen) (nec:quic_protect k l) (nl:pnlen) :
+  epn nl * cipher (fst k) (l-nl) 
+
+val sample_quic_protect (#k:quicid) (#l:pnplainlen) (nec:quic_protect k l) : PNE.sample
+
+#reset-options "--z3rlimit 50"
 
 
 val encrypt
-  (#i:I.id)
-  (#j:I.id)
-  (w:stream_writer i j)
-  (nl:pnlen)
-  (l:plainLen)
-  (p:plain i l):
-  ST ((epn nl) * (cipher i l))
-  (requires fun h0 -> wincrementable w h0 /\ invariant w h0)
-  (ensures fun h0 (ne,c) h1 ->
+  (#k:quicid)
+  (w:stream_writer k)
+  (#hl:headerlen)
+  (hd:quic_header k hl)
+  (nl:pnlen {hl + nl <= v AEAD.aadmax})
+  (#l:plainlen {hl + nl + l + v AEAD.taglen <= pow2 32 - 1 /\
+    nl + l + v AEAD.taglen >= samplelen + 4})
+  (p:plain (fst k) l):
+  ST (quic_packet k hl (nl + l))
+  (requires fun h0 ->
+    wincrementable w h0 /\
+    invariant w h0)
+  (ensures fun h0 (ph,nec) h1 ->
+    let (i,j) = k in
     let aw = writer_aead_state w in
     let ps = writer_pne_state w in
     invariant w h1 /\
     wctrT w h1 == wctrT w h0 + 1 /\ 
-    ((Flag.safePNE j /\ Flag.safeId i) ==> (
+    (safeQUIC k ==> (
+      let (ne,c) = split #k #(nl+l) nec nl in
       let rpn = rpn_of_nat (wctrT w h0) in
       let npn = npn_encode j rpn nl in
-      let s = PNE.sample_cipher c in
       let alg = I.cipherAlg_of_aeadAlg ((AEAD.wgetinfo aw).AEAD.alg) in
-      let n = create_nonce #i #alg (writer_iv w) nl rpn in
-      let ad = Bytes.empty_bytes in
-      AEAD.wlog aw h1 == Seq.snoc (AEAD.wlog aw h0) (AEAD.Entry #i #(AEAD.wgetinfo aw) #nl n ad p c) /\
-      PNE.table ps h1 == Seq.snoc (PNE.table ps h0) (PNE.Entry #j #npn_pkg s #nl ne npn))) /\
+      let nce:AEAD.nonce (AEAD.wgetinfo aw) = create_nonce #i #alg (writer_iv w) rpn in
+      let ad:AEAD.adata = Bytes.append (bytes_of_quic_header hd) npn in
+      let s:PNE.sample = sample_quic_protect nec in
+      let nn = pne_plain_of_header_pn hd npn in
+      let cc = pne_cipher_of_pheader_epn ph ne in 
+      AEAD.wlog aw h1 ==
+        Seq.snoc
+          (AEAD.wlog aw h0)
+          (AEAD.Entry #i #(AEAD.wgetinfo aw) nce ad #l p c) /\
+           PNE.table ps h1 ==
+              Seq.snoc
+                (PNE.table ps h0)
+                (PNE.Entry #j #pne_plain_pkg s #(nl+1) nn cc))) /\
     modifies (Set.union (footprint w) (shared_footprint w)) h0 h1)
 
 
 
-#reset-options "--z3rlimit 50"
-
 val decrypt
-  (#i:I.id)
-  (#j:I.id)
-  (#w:stream_writer i j)
+  (#k:quicid)
+  (#w:stream_writer k)
   (r:stream_reader w)
-  (#nl:pnlen)
-  (ne:epn nl)
-  (l:plainLen)
-  (c:cipher i l):
-  ST (option (plain i l))
+  (#hl:headerlen {hl+5 <= v AEAD.aadmax})
+  (#nll:pnplainlen{hl + nll + v AEAD.taglen <= pow2 32 - 1})
+  (qp:quic_packet k hl nll) :
+  ST (option (l:plainlen & plain (fst k) l))
   (requires fun h0 -> rinvariant r h0 /\ invariant w h0)
   (ensures fun h0 res h1 ->
+    let (i,j) = k in
     let ar = reader_aead_state r in
     let aw = writer_aead_state w in
     let ps = reader_pne_state r in
     rinvariant r h1 /\
     modifies (Set.union (rfootprint r) (rshared_footprint r)) h0 h1 /\
-    (None? res ==> expected_pnT r h1 == expected_pnT r h0) /\    
-    ((Flag.safePNE j /\ Flag.safeId i) ==> 
-      (let s = PNE.sample_cipher c in
-      match PNE.entry_for_sample_epn s ne ps h0 with
+    (None? res ==> expected_pnT r h1 == expected_pnT r h0) /\
+    (safeQUIC k ==>
+      (let (ph,nec) = qp in
+      let s = sample_quic_protect nec in
+      let cp = pne_cipherpad_of_pheader_quicprotect ph nec in
+      match PNE.entry_for_sample_cipherpad s cp ps h0 with
         | None -> None? res
-        | Some (PNE.Entry  _ _ npn) ->
+        | Some (PNE.Entry  _ #ll n cc) ->
+          let nl:pnlen = ll - 1 in
+          let (hd,npn) = header_pn_of_pne_plain #k #hl ph #ll n in 
 	  let rpn = npn_decode #j #nl npn (expected_pnT r h0) in
           let alg = I.cipherAlg_of_aeadAlg ((AEAD.rgetinfo ar).AEAD.alg) in
-          let n = create_nonce #i #alg (reader_iv r) nl rpn in
-          match AEAD.wentry_for_nonce aw #nl n h0 with
+          let n = create_nonce #i #alg (reader_iv r) rpn in
+          let ad:AEAD.adata = Bytes.append (bytes_of_quic_header hd) npn in
+          match AEAD.wentry_for_nonce aw n h0 with
 	    | None -> None? res
 	    | Some (AEAD.Entry _  ad' #l' p' c')  -> 
-	      if ad' = Bytes.empty_bytes && l' = l && c' = c then 
-	        (res = Some p' /\
+	      if ad' = ad && l' = nll - nl && snd (split nec nl) = c' then 
+	        (res = Some (|l',p'|) /\
                   (if U64.v rpn >= U64.v (expected_pnT r h0) && U64.v rpn < max_ctr then
                     expected_pnT r h1 = rpn_of_nat (U64.v rpn + 1)
                   else
@@ -344,7 +406,7 @@ val decrypt
     nl:pnlen ->
     pn:rpn ->
     ad:AEAD.adata ->
-    #l:plainLen ->
+    #l:plainlen ->
     p:plain i l ->
     ne:epn nl ->
     c:cipher i l ->
